FixIsMu/LogRelFI/LemmasPseudoType.v
@@ -1,3 +1,5 @@
+Require StlcIso.TypeSafety.
+Require Import StlcIso.LemmasTyping.
 Require Import StlcFix.CanForm.
 Require Import StlcFix.LemmasTyping.
 (* Require Import StlcIso.LemmasScoping. *)
@@ -25,11 +27,22 @@ Ltac crushRepEmulEmbed :=
     | [ |- context[ repEmulCtx( embedCtx ?Γ) ] ] => rewrite -> (repEmulCtx_embedCtx_leftinv Γ)
   end.
 
+(* TODO: equivalent section for fxToIs? *)
+
 Lemma getevar_repEmulCtx {i τ Γ} :
   ⟪ i : τ ∈ repEmulCtx Γ ⟫ →
   exists τ', ⟪ i : τ' p∈ Γ ⟫ ∧ τ = repEmul τ'.
 Proof.
-  revert i. induction Γ as [|Γ IHΓ τ'']; 
+  revert i. induction Γ as [|Γ IHΓ τ''];
+  inversion 1; [idtac| destruct (IHΓ _ H4) as [? [? ?]]];
+  eauto using GetEvarP.
+Qed.
+
+Lemma getevar_fxToIsCtx {i τ Γ} :
+  ⟪ i : τ i∈ fxToIsCtx Γ ⟫ →
+  exists τ', ⟪ i : τ' p∈ Γ ⟫ ∧ τ = fxToIs τ'.
+Proof.
+  revert i. induction Γ as [|Γ IHΓ τ''];
   inversion 1; [idtac| destruct (IHΓ _ H4) as [? [? ?]]];
   eauto using GetEvarP.
 Qed.
@@ -40,11 +53,10 @@ Section OfType.
     unfold OfType, OfTypeStlcFix, OfTypeStlcIso; intros;
     repeat
       (subst;
-       stlcCanForm;
-       crushTyping;
-       I.crushTyping;
+       F.stlcCanForm;
+       I.stlcCanForm;
        F.crushTyping;
-       (* crushUtlcScoping; *)
+       I.crushTyping;
        destruct_conjs;
        repeat
          match goal with
@@ -84,8 +96,8 @@ Section OfType.
 
   Lemma OfType_lambda {τ₁ τ₂ τ₁' tsb tub} :
     τ₁' = repEmul τ₁ →
-    I.Typing I.empty (I.abs (fxToIs τ₁) tub) (I.tarr (fxToIs τ₁) (fxToIs τ₂)) →
-    ⟪ empty ⊢ F.abs (repEmul τ₁) tsb : repEmul τ₁ ⇒ repEmul τ₂ ⟫ →
+    ⟪ I.empty i⊢ I.abs (fxToIs τ₁) tub : I.tarr (fxToIs τ₁) (fxToIs τ₂) ⟫ →
+    ⟪ F.empty ⊢ F.abs (repEmul τ₁) tsb : repEmul τ₁ ⇒ repEmul τ₂ ⟫ →
     OfType (ptarr τ₁ τ₂) (F.abs τ₁' tsb) (I.abs (fxToIs τ₁) tub).
   Proof. crush. Qed.
 
@@ -93,103 +105,95 @@ Section OfType.
     OfType ptunit ts tu →
     ts = F.unit ∧ tu = I.unit.
   Proof.
-    intros.
-    inversion H.
-    unfold OfTypeStlcFix in H0.
-    inversion H1.
     crush.
-    inversion H0.
-    inversion H.
   Qed.
 
-  Lemma OfType_inversion_ptbool {ts tu} :
-    OfType ptbool ts tu →
-    ts = S.true ∧ tu = U.true ∨
-    ts = S.true ∧ tu = U.false ∨
-    ts = S.false ∧ tu = U.true ∨
-    ts = S.false ∧ tu = U.false.
-  Proof. crush. Qed.
+  (* Lemma OfType_inversion_ptbool {ts tu} : *)
+  (*   OfType ptbool ts tu → *)
+  (*   ts = S.true ∧ tu = U.true ∨ *)
+  (*   ts = S.true ∧ tu = U.false ∨ *)
+  (*   ts = S.false ∧ tu = U.true ∨ *)
+  (*   ts = S.false ∧ tu = U.false. *)
+  (* Proof. crush. Qed. *)
 
   Lemma OfType_inversion_ptsum {τ₁ τ₂ ts tu} :
     OfType (ptsum τ₁ τ₂) ts tu →
     ∃ ts' tu',
-      ts = S.inl ts' ∧ tu = U.inl tu' ∧ OfType τ₁ ts' tu' ∨
-      ts = S.inl ts' ∧ tu = U.inr tu' ∨
-      ts = S.inr ts' ∧ tu = U.inl tu' ∨
-      ts = S.inr ts' ∧ tu = U.inr tu' ∧ OfType τ₂ ts' tu'.
-  Proof. crush. Qed.
+      ts = F.inl ts' ∧ tu = I.inl tu' ∧ OfType τ₁ ts' tu' ∨
+      ts = F.inl ts' ∧ tu = I.inr tu' ∨
+      ts = F.inr ts' ∧ tu = I.inl tu' ∨
+      ts = F.inr ts' ∧ tu = I.inr tu' ∧ OfType τ₂ ts' tu'.
+  Proof.
+    crush.
+  Qed.
 
-  Lemma OfType_inversion_ptprod {τ₁ τ₂ ts tu} :
-    OfType (ptprod τ₁ τ₂) ts tu →
-    ∃ ts₁ tu₁ ts₂ tu₂,
-      ts = S.pair ts₁ ts₂ ∧
-      tu = U.pair tu₁ tu₂ ∧
-      OfType τ₁ ts₁ tu₁ ∧
-      OfType τ₂ ts₂ tu₂.
-  Proof. crush. Qed.
+  (* Lemma OfType_inversion_ptprod {τ₁ τ₂ ts tu} : *)
+  (*   OfType (ptprod τ₁ τ₂) ts tu → *)
+  (*   ∃ ts₁ tu₁ ts₂ tu₂, *)
+  (*     ts = S.pair ts₁ ts₂ ∧ *)
+  (*     tu = U.pair tu₁ tu₂ ∧ *)
+  (*     OfType τ₁ ts₁ tu₁ ∧ *)
+  (*     OfType τ₂ ts₂ tu₂. *)
+  (* Proof. crush. Qed. *)
 
-  Lemma OfTypeUtlc_inversion_ptarr {τ₁ τ₂ tu} :
-    OfTypeUtlc (ptarr τ₁ τ₂) tu →
-    ∃ tu', tu = U.abs tu' ∧ ⟨ 1 ⊢ tu' ⟩.
-  Proof. crush. Qed.
+  (* Lemma OfTypeUtlc_inversion_ptarr {τ₁ τ₂ tu} : *)
+  (*   OfTypeUtlc (ptarr τ₁ τ₂) tu → *)
+  (*   ∃ tu', tu = U.abs tu' ∧ ⟨ 1 ⊢ tu' ⟩. *)
+  (* Proof. crush. Qed. *)
 
-  Lemma OfTypeUtlc_inversion_ptprod {τ₁ τ₂ tu} :
-    OfTypeUtlc (ptprod τ₁ τ₂) tu →
-    ∃ tu₁ tu₂, tu = U.pair tu₁ tu₂ ∧ OfTypeUtlc τ₁ tu₁ ∧ OfTypeUtlc τ₂ tu₂.
-  Proof. crush. Qed.
+  (* Lemma OfTypeUtlc_inversion_ptprod {τ₁ τ₂ tu} : *)
+  (*   OfTypeUtlc (ptprod τ₁ τ₂) tu → *)
+  (*   ∃ tu₁ tu₂, tu = U.pair tu₁ tu₂ ∧ OfTypeUtlc τ₁ tu₁ ∧ OfTypeUtlc τ₂ tu₂. *)
+  (* Proof. crush. Qed. *)
 
-  Lemma OfTypeUtlc_inversion_ptsum {τ₁ τ₂ tu} :
-    OfTypeUtlc (ptsum τ₁ τ₂) tu →
-    ∃ tu', (tu = U.inl tu' ∧ OfTypeUtlc τ₁ tu') ∨
-           (tu = U.inr tu' ∧ OfTypeUtlc τ₂ tu').
-  Proof. crush. Qed.
+  (* Lemma OfTypeUtlc_inversion_ptsum {τ₁ τ₂ tu} : *)
+  (*   OfTypeUtlc (ptsum τ₁ τ₂) tu → *)
+  (*   ∃ tu', (tu = U.inl tu' ∧ OfTypeUtlc τ₁ tu') ∨ *)
+  (*          (tu = U.inr tu' ∧ OfTypeUtlc τ₂ tu'). *)
+  (* Proof. crush. Qed. *)
 
   Lemma OfType_inversion_ptarr {τ₁ τ₂ ts tu} :
     OfType (ptarr τ₁ τ₂) ts tu →
     ∃ ts' tu',
-      ts = S.abs (repEmul τ₁) ts' ∧
-      tu = U.abs tu' ∧
+      ts = F.abs (repEmul τ₁) ts' ∧
+      tu = I.abs (fxToIs τ₁) tu' ∧
       ⟪ empty ▻ repEmul τ₁ ⊢ ts' : repEmul τ₂ ⟫ ∧
-      ⟨ 1 ⊢ tu' ⟩.
+      I.Typing (I.evar I.empty (fxToIs τ₁)) tu' (fxToIs τ₂).
   Proof. crush. Qed.
 
-  Lemma OfType_inversion_pEmulDV {n p ts tu} :
-    OfType (pEmulDV n p) ts tu →
-    S.Value ts ∧ U.Value tu ∧
-    ⟪ empty ⊢ ts : UVal n ⟫ ∧
-    ⟨ 0 ⊢ tu ⟩.
+  Lemma OfType_inversion_pEmulDV {n p ts tu T} :
+    OfType (pEmulDV n p T) ts tu →
+    F.Value ts ∧ I.Value tu ∧
+    ⟪ empty ⊢ ts : UValFI n T ⟫ ∧
+    I.Typing I.empty tu T.
   Proof. crush. Qed.
 
-  Lemma OfTypeUtlc'_implies_Value {τ tu} :
-    OfTypeUtlc' τ tu →
-    U.Value tu.
+  Lemma OfTypeStlcIso_implies_Value {τ tu} :
+    OfTypeStlcIso τ tu →
+    I.Value tu.
   Proof.
-    revert tu.
-    induction τ; crush.
+    crush.
   Qed.
 
-  Lemma OfTypeUtlc_implies_Value {τ tu} :
-    OfTypeUtlc τ tu →
-    U.Value tu.
+  Lemma OfTypeStlcFix_implies_Value {τ ts} :
+    OfTypeStlcFix τ ts →
+    F.Value ts.
   Proof.
-    destruct 1 as (ctu & otu).
-    eauto using OfTypeUtlc'_implies_Value.
+    crush.
   Qed.
 
   Lemma OfType_implies_Value {τ ts tu} :
     OfType τ ts tu →
-    S.Value ts ∧ U.Value tu.
+    F.Value ts ∧ I.Value tu.
   Proof.
-    unfold OfType, OfTypeStlc.
-    intros ot; destruct_conjs;
-    eauto using OfTypeUtlc_implies_Value.
+    crush.
   Qed.
 
-  Lemma OfType_pEmulDV {n p ts tu} :
-    S.Value ts ∧ U.Value tu ∧
-    ⟪ empty ⊢ ts : UVal n ⟫ → 
-    ⟨ 0 ⊢ tu ⟩ →
-    OfType (pEmulDV n p) ts tu.
+  Lemma OfType_pEmulDV {n p ts tu T} :
+    F.Value ts ∧ I.Value tu ∧
+    ⟪ empty ⊢ ts : UValFI n T ⟫ →
+    I.Typing I.empty tu T →
+    OfType (pEmulDV n p T) ts tu.
   Proof. crush. Qed.
 
 End OfType.
@@ -198,25 +202,25 @@ Ltac crushOfType :=
   repeat
     match goal with
       | [ H: OfType ptunit _ _ |- _ ] => apply OfType_inversion_ptunit in H
-      | [ H: OfType ptbool _ _ |- _ ] => apply OfType_inversion_ptbool in H
+      (* | [ H: OfType ptbool _ _ |- _ ] => apply OfType_inversion_ptbool in H *)
       | [ H: OfType (ptsum _ _) _ _ |- _ ] => apply OfType_inversion_ptsum in H
-      | [ H: OfType (ptprod _ _) _ _ |- _ ] => apply OfType_inversion_ptprod in H
+      (* | [ H: OfType (ptprod _ _) _ _ |- _ ] => apply OfType_inversion_ptprod in H *)
       | [ H: OfType (ptarr _ _) _ _ |- _ ] => apply OfType_inversion_ptarr in H
-      | [ H: OfTypeUtlc _ ?t |- ⟨ 0 ⊢ ?t ⟩ ] => exact (proj1 H)
-      | [ H: OfTypeUtlc ?τ ?t |- OfTypeUtlc' ?τ ?t ] => exact (proj2 H)
-      | [ H: OfTypeUtlc (ptarr _ _) _ |- _ ] => apply OfTypeUtlc_inversion_ptarr in H
-      | [ H: OfTypeUtlc (ptprod _ _) _ |- _ ] => apply OfTypeUtlc_inversion_ptprod in H
-      | [ H: OfTypeUtlc (ptsum _ _) _ |- _ ] => apply OfTypeUtlc_inversion_ptsum in H
-      | [ H: OfType (pEmulDV _ _) _ _ |- _ ] => apply OfType_inversion_pEmulDV in H
+      (* | [ H: OfTypeUtlc _ ?t |- ⟨ 0 ⊢ ?t ⟩ ] => exact (proj1 H) *)
+      (* | [ H: OfTypeUtlc ?τ ?t |- OfTypeUtlc' ?τ ?t ] => exact (proj2 H) *)
+      (* | [ H: OfTypeUtlc (ptarr _ _) _ |- _ ] => apply OfTypeUtlc_inversion_ptarr in H *)
+      (* | [ H: OfTypeUtlc (ptprod _ _) _ |- _ ] => apply OfTypeUtlc_inversion_ptprod in H *)
+      (* | [ H: OfTypeUtlc (ptsum _ _) _ |- _ ] => apply OfTypeUtlc_inversion_ptsum in H *)
+      (* | [ H: OfType (pEmulDV _ _) _ _ |- _ ] => apply OfType_inversion_pEmulDV in H *)
       (* | [ H: OfTypeUtlc ptbool ?t  |- _ ] =>  change (OfTypeUtlc ptbool t) with (t = U.true ∨ t = U.false) in H *)
       (* | [ H: OfTypeUtlc ptunit ?t  |- _ ] => change (OfTypeUtlc ptunit t) with (t = U.unit) in H; subst t *)
-      | [ |- OfType ptunit S.unit U.unit ] => apply OfType_unit
-      | [ |- OfType ptbool S.true U.true ] => apply OfType_true
-      | [ |- OfType ptbool S.false U.false ] => apply OfType_false
-      | [ |- OfType (ptsum _ _) (S.inl _) (U.inl _)] => apply OfType_inl
-      | [ |- OfType (ptsum _ _) (S.inr _) (U.inr _)] => apply OfType_inr
-      | [ |- OfType (ptprod _ _) (S.pair _ _) (U.pair _ _) ] => apply OfType_pair
-      | [ |- OfType (ptarr _ _) (S.abs _ _) (U.abs _) ] => apply OfType_lambda
-      | [ |- OfTypeUtlc _ _ ] => split
-      | [ |- OfType (pEmulDV _ _) _ _ ] => apply OfType_pEmulDV
+      | [ |- OfType ptunit F.unit I.unit ] => apply OfType_unit
+      (* | [ |- OfType ptbool S.true U.true ] => apply OfType_true *)
+      (* | [ |- OfType ptbool S.false U.false ] => apply OfType_false *)
+      | [ |- OfType (ptsum _ _) (F.inl _) (I.inl _)] => apply OfType_inl
+      | [ |- OfType (ptsum _ _) (F.inr _) (I.inr _)] => apply OfType_inr
+      (* | [ |- OfType (ptprod _ _) (S.pair _ _) (U.pair _ _) ] => apply OfType_pair *)
+      | [ |- OfType (ptarr _ _) (F.abs _ _) (I.abs _ _) ] => apply OfType_lambda
+      (* | [ |- OfTypeUtlc _ _ ] => split *)
+      | [ |- OfType (pEmulDV _ _ _) _ _ ] => apply OfType_pEmulDV
     end.
