FixIsMu/StlcFix/SpecSyntax.v
@@ -8,6 +8,7 @@ Inductive Ty : Set :=
   (* | tprod (τ₁ τ₂: Ty) *)
   | tsum (τ₁ τ₂: Ty).
 
+
 Notation "A ⊎ B" := (tsum A B) (at level 85, right associativity).
 (* Notation "A × B" := (tprod A B) (at level 85, right associativity). *)
 Notation "A ⇒ B" := (tarr A B) (at level 85, right associativity).
