FixIsMu/StlcIso/Contraction.v
@@ -1,0 +1,799 @@
+Require Export StlcIso.Inst.
+Require Export StlcIso.SpecSyntax.
+Require Export StlcIso.SpecTyping.
+Require Coq.Program.Tactics.
+Require Coq.Program.Wf.
+Require Coq.Arith.Wf_nat.
+Require Import Coq.Logic.FunctionalExtensionality.
+
+Require Import FunInd.
+Require Import Recdef.
+Require Import Db.Lemmas.
+
+Require Import Lia.
+
+Fixpoint LMC (τ : Ty) {struct τ} : nat :=
+  match τ with
+  | trec τ => S (LMC τ)
+  | _ => 0
+  end.
+
+Inductive Contr : Ty → Prop :=
+  | ContrPrim : Contr tunit
+  | ContrArr {τ τ'} : Contr (tarr τ τ')
+  | ContrSum {τ τ'} : Contr (tsum τ τ')
+  | ContrRec {τ} :
+      Contr τ →
+      Contr (trec τ).
+
+Lemma lmc_invar_subst : ∀ (τ : Ty) (ξ : Sub Ty), Contr τ → LMC τ = LMC (τ[ξ]).
+Proof.
+  intros.
+  revert ξ.
+  induction H.
+  constructor.
+  constructor.
+  constructor.
+  simpl.
+  intros.
+  specialize (IHContr ξ↑).
+  eauto.
+Qed.
+
+Lemma contr_implies_contr_unroll (τ : Ty) (P : Contr (trec τ)) : Contr (τ[beta1 (trec τ)]).
+  inversion P.
+  subst.
+  (* Clear out hypothesis so it dosn't mess up the induction *)
+  clear P.
+  (* Generalize the substitution *)
+  remember (beta1 (trec τ)) as ξ.
+  (* Get rid of equality so induction is general (and thus IH is stronger) *)
+  clear Heqξ.
+  (* Put ξ back in goal so it is inducted upon *)
+  revert ξ.
+  induction H0;
+  constructor.
+  apply IHContr.
+Qed.
+
+Program Fixpoint fu (τ : Ty) (P : Contr τ) {measure (LMC τ)} : Ty :=
+  match τ with
+  | trec τ' => fu τ'[beta1 (trec τ')] _
+  | _ => τ
+  end.
+Next Obligation.
+  exact (contr_implies_contr_unroll τ' P).
+Qed.
+Next Obligation.
+  inversion P.
+  rewrite <- ?(lmc_invar_subst τ' (beta1 (trec τ')) H0).
+  constructor.
+Qed.
+
+
+Fixpoint fu_accum (τ : Ty) (current_sub : Sub Ty) {struct τ} : Ty :=
+  match τ with
+    | trec τ => fu_accum τ (comp (up current_sub) (beta1 (trec τ)[current_sub]))
+    | _ => τ[current_sub]
+  end.
+
+Definition fu' (τ : Ty) := fu_accum τ (idm Ty).
+
+
+Eval compute in (fu' (trec (tsum (tvar 0) tunit))).
+Eval compute in (fu' (trec (trec (tsum (tvar 0) tunit)))).
+Compute (fu' (trec (trec (tsum (tvar 1) (tvar 0))))).
+
+Functional Scheme fu_accum_ind := Induction for fu_accum Sort Prop.
+Functional Scheme lmc_ind := Induction for LMC Sort Prop.
+(* Functional Scheme fu_func_ind := Induction for fu_func Sort Prop. *)
+
+(* Check fu_ind. *)
+
+
+Lemma contr_implies_contr_fu (τ : Ty) (P : Contr τ) : Contr (fu' τ).
+Proof.
+  unfold fu'.
+  generalize (idm Ty).
+  induction P; cbn;
+  constructor || intuition.
+Qed.
+
+(* simple recursive type: *)
+(*   α | τ_contr *)
+
+
+(* τ_contr: *)
+(* tunit *)
+(* simple => simple *)
+(* μ α . τ_contr *)
+
+
+
+Inductive SimpleContr : Ty → Prop :=
+| SimpContrPrim : SimpleContr tunit
+| SimpContrArrow {τ τ'} : SimpleRec τ → SimpleRec τ' → SimpleContr (tarr τ τ')
+| SimpContrSum {τ τ'} : SimpleRec τ → SimpleRec τ' → SimpleContr (tsum τ τ')
+| SimpContrRec {τ} : SimpleContr τ → SimpleContr (trec τ)
+with SimpleRec : Ty → Prop :=
+| SimpleAlpha {i} : SimpleRec (tvar i)
+| SimpleRecContr {τ} : SimpleContr τ → SimpleRec τ.
+
+Scheme simp_contr_mut_ind := Induction for SimpleContr Sort Prop
+  with simp_rec_mut_ind := Induction for SimpleRec Sort Prop.
+
+Combined Scheme simp_contr_comb_ind from simp_contr_mut_ind, simp_rec_mut_ind.
+
+Definition SimpleContrSub (ξ : Sub Ty) : Prop := forall i : Ix, SimpleContr (ξ i).
+Definition SimpleRecSub (ξ : Sub Ty) : Prop := forall i : Ix, SimpleRec (ξ i).
+
+Lemma SimpleContrSub_implies_SimpleRecSub {ξ} : SimpleContrSub ξ → SimpleRecSub ξ.
+Proof.
+  unfold SimpleContrSub, SimpleRecSub.
+  intros.
+  specialize (H i).
+  exact (SimpleRecContr H).
+Qed.
+
+Lemma SimpleContrSub_comp {ξ δ} : SimpleContrSub ξ → SimpleContrSub (δ >-> ξ).
+Proof.
+  unfold SimpleContrSub.
+  intros.
+  unfold fcomp.
+  exact (H (δ i)).
+Qed.
+
+Lemma SimpleRecSub_comp {ξ δ} : SimpleRecSub ξ → SimpleRecSub (δ >-> ξ).
+Proof.
+  unfold SimpleRecSub.
+  intros.
+  unfold fcomp.
+  exact (H (δ i)).
+Qed.
+
+Lemma SimpleContr_implies_SimpleRec {τ} : SimpleContr τ → SimpleRec τ.
+Proof.
+  apply SimpleRecContr.
+Qed.
+
+Lemma SimpleRecSub_wkm : SimpleRecSub wkm.
+Proof.
+  unfold SimpleRecSub; cbn; constructor.
+Qed.
+
+Lemma SimpleRec_implies_SimpleRecSub_snoc {ξ τ} : SimpleRecSub ξ → SimpleRec τ → SimpleRecSub (ξ · τ).
+Proof.
+  unfold SimpleRecSub, snoc.
+  intros.
+  destruct i;
+  intuition.
+Qed.
+
+Lemma SimpleContr_implies_SimpleContrSub_snoc {ξ τ} : SimpleContrSub ξ → SimpleContr τ → SimpleContrSub (ξ · τ).
+Proof.
+  unfold SimpleContrSub, snoc.
+  intros.
+  destruct i;
+  intuition.
+Qed.
+
+(* Lemma SimpleRecSub_Left_comp {ξ δ} : SimpleRecSub ξ → SimpleRecSub (ξ >-> δ). *)
+(* Proof. *)
+(*   unfold SimpleRecSub. *)
+(*   intros. *)
+(*   cbn. *)
+(*   specialize (H i). *)
+(*   inversion H. *)
+
+Compute (wk (trec (tsum tunit (tvar 0)))).
+Compute (wk tunit).
+Compute (wk (tarr tunit (tvar 0))).
+Compute ((tvar 0)[wk↑]).
+Compute ((tvar 1)[wk↑]).
+
+(* Due to definition of wk and up this seems to be cyclic with SimpleRecSubUp *)
+Lemma SimpleRec_wk {τ} : SimpleRec τ → SimpleRec τ[wk]
+with SimpleContr_wk {τ} : SimpleContr τ → SimpleContr τ[wk].
+Proof.
+  (* change τ[wk] with (wk τ). *)
+  (* rewrite ap_wk. *)
+  (* intros. *)
+
+  induction τ; cbn; intros;
+  repeat change (apTy ?ξ ?τ) with τ[ξ].
+
+  inversion H.
+  inversion H0.
+  specialize (IHτ1 H4).
+  specialize (IHτ2 H5).
+  constructor.
+  constructor; assumption.
+
+  constructor.
+  constructor.
+
+  inversion H.
+  inversion H0.
+  specialize (IHτ1 H4).
+  specialize (IHτ2 H5).
+  constructor.
+  constructor; assumption.
+
+  (* constructor. *)
+  (* constructor. *)
+
+
+  (* apply SimpleRec_implies_SimpleRecSub_snoc. *)
+
+
+  (* inversion H. *)
+  (* inversion H0. *)
+  (* pose proof (SimpleRecContr H3). *)
+  (* specialize (IHτ H4). *)
+  (* constructor. *)
+  (* constructor. *)
+
+  (* (* remember wk↑ as ξ. *) *)
+  (* rewrite <- ap_wk. *)
+  (* unfold up. *)
+
+Admitted.
+  (* apply SimpleRec_implies_SimpleRecSub_snoc. *)
+  (* assumption. *)
+  (* unfold up, fcomp, snoc. *)
+  (* change ?τ[?ξ] with (apTy ξ τ). *)
+  (* unfold apTy. *)
+  (* destruct Heqξ. *)
+  (* unfold fcomp. *)
+  (* unfold snoc. *)
+
+(* Admitted. *)
+  (* extensionality i. *)
+
+
+
+
+  (* apply (simp_rec_mut_ind *)
+  (*          (fun {τ} (_ : SimpleContr τ) => (SimpleContr τ → SimpleContr τ[wk])) *)
+  (*          (fun {τ} (_ : SimpleRec τ) => (SimpleRec τ → SimpleRec τ[wk]))); *)
+  (*   cbn; intros. *)
+  (* constructor. *)
+  (* inversion H1. *)
+  (* constructor; intuition. *)
+  (* inversion H1. *)
+  (* constructor; intuition. *)
+  (* crushDbSyntaxMatchH. *)
+  (* constructor. *)
+  (* unfold up. *)
+  (* Admitted. *)
+
+(*   unfold apTy. *)
+(*   apply SimpleRec_implies_SimpleRecSub_snoc. *)
+(*   induction τ0; cbn. *)
+
+
+(*   crushRewriter. *)
+(*   destruct τ; cbn. *)
+(*   4: { *)
+(*     crushRewriter. *)
+(*     crushDbLemmasRewriteH. *)
+(*     crushDbLemmasMatchH. *)
+(*   } *)
+
+
+
+(*   induction 1; cbn. *)
+(*   constructor. *)
+(*   inversion H. *)
+(*   4: { *)
+(*     crushDbLemmasRewriteH. *)
+(*     cbn. *)
+(*     constructor. *)
+(*     constructor. *)
+(*   } *)
+
+
+(*   induction τ. *)
+(*   constructor; constructor; assumption. *)
+(*   constructor; constructor. *)
+(*   constructor; constructor; assumption. *)
+(*   constructor; constructor. *)
+
+(* Lemma SimpleContr_wk {τ} : SimpleContr τ → SimpleContr τ[wk]. *)
+(* Proof. *)
+(*   apply (simp_contr_mut_ind *)
+(*            (fun {τ} (_ : SimpleContr τ) => (SimpleContr τ → SimpleContr τ[wk])) *)
+(*            (fun {τ} (_ : SimpleRec τ) => (SimpleRec τ → SimpleRec τ[wk]))); *)
+(*     cbn; intros. *)
+(*   constructor. *)
+(*   inversion H1. *)
+(*   constructor; intuition. *)
+(*   inversion H1. *)
+(*   constructor; intuition. *)
+(*   crushDbSyntaxMatchH. *)
+(*   constructor. *)
+(*   specialize (H s). *)
+(*   repeat change (apTy ?ξ ?τ) with τ[ξ]. *)
+(* Admitted. *)
+
+
+Lemma SimpleRecSub_implies_SimpleRecSubUp {ξ} : SimpleRecSub ξ → SimpleRecSub (up ξ).
+Proof.
+  unfold SimpleRecSub.
+  intros.
+
+  destruct i; cbn.
+  constructor.
+
+  apply SimpleRec_wk.
+  exact (H i).
+Qed.
+
+(* Lemma SimpleContrSub_implies_SimpleRecSubUp {ξ} : SimpleContrSub ξ → SimpleContrSub (up ξ). *)
+(* Proof. *)
+(*   unfold up. *)
+(*   intros. *)
+(*   apply SimpleContr_implies_SimpleContrSub_snoc. *)
+(*   unfold fcomp, SimpleContrSub in *. *)
+(*   intros. *)
+(*   apply SimpleContr_wk. *)
+(*   intuition. *)
+(*   cbn. *)
+(*   constructor. *)
+(* Qed. *)
+
+Lemma SimpleRecSub_implies_SimpleRec {τ ξ} : SimpleRec τ → SimpleRecSub ξ → SimpleRec τ[ξ].
+Proof.
+  intro H.
+  apply (simp_rec_mut_ind
+           (fun {τ} (_ : SimpleContr τ) => (forall ξ : Sub Ty, SimpleRecSub ξ → SimpleContr τ[ξ]))
+           (fun {τ} (_ : SimpleRec τ) => (forall ξ : Sub Ty, SimpleRecSub ξ → SimpleRec τ[ξ]))).
+  cbn.
+  constructor.
+  cbn.
+  intros.
+  constructor; intuition.
+  apply H0.
+  assumption.
+  apply H1.
+  assumption.
+  cbn.
+  intros.
+  constructor; intuition.
+  apply H0.
+  assumption.
+  apply H1.
+  assumption.
+  cbn.
+  intros.
+  constructor.
+  eauto using H0, SimpleRecSub_implies_SimpleRecSubUp.
+
+  intros.
+  apply H0.
+
+  intros.
+  eauto using SimpleRecContr.
+
+  assumption.
+Qed.
+
+Check simp_contr_mut_ind.
+
+Lemma SimpleContrSub_implies_SimpleContr {τ ξ} : SimpleContr τ → SimpleRecSub ξ → SimpleContr τ[ξ].
+  intro H.
+  apply (simp_contr_mut_ind
+           (fun {τ} (_ : SimpleContr τ) => (forall ξ : Sub Ty, SimpleRecSub ξ → SimpleContr τ[ξ]))
+           (fun {τ} (_ : SimpleRec τ) => (forall ξ : Sub Ty, SimpleRecSub ξ → SimpleRec τ[ξ]))).
+  cbn.
+  constructor.
+
+  intros.
+  cbn.
+  constructor.
+  apply H0.
+  assumption.
+  apply H1.
+  assumption.
+
+  intros.
+  cbn.
+  constructor.
+  apply H0.
+  assumption.
+  apply H1.
+  assumption.
+
+  intros.
+  cbn.
+  constructor.
+  apply H0.
+  apply SimpleRecSub_implies_SimpleRecSubUp.
+  assumption.
+
+  intros.
+  cbn.
+  exact (H0 i).
+
+  intros.
+  specialize (H0 ξ0).
+  apply SimpleRecSub_implies_SimpleRec.
+  apply SimpleRecContr.
+  assumption.
+
+  assumption.
+  assumption.
+Qed.
+
+Lemma idm_contr_sub : SimpleRecSub (idm Ty).
+Proof.
+  unfold SimpleRecSub; cbn.
+  constructor.
+Qed.
+
+Lemma SimpleRecSub_compose {ξ ζ} : SimpleRecSub ξ → SimpleRecSub ζ → SimpleRecSub (ξ >=> ζ).
+Proof.
+  unfold SimpleRecSub.
+  intros.
+  unfold comp.
+  unfold ap.
+  cbn.
+  apply SimpleRecSub_implies_SimpleRec.
+  exact (H i).
+  assumption.
+Qed.
+
+Lemma simpl_contr_implies_contr_fu {τ} : SimpleContr τ → SimpleContr (fu' τ)
+with simpl_rec_implies_rec_fu {τ} : SimpleRec τ → SimpleRec (fu' τ).
+Proof.
+  - unfold fu'.
+    intro P.
+    pose proof idm_contr_sub.
+    revert H.
+    generalize (idm Ty).
+    (* functional induction (fu_accum τ ξ) using fu_accum_ind. *)
+    intros ξ Q.
+
+    functional induction (fu_accum τ ξ) using fu_accum_ind; cbn.
+    inversion P.
+    constructor;
+    apply SimpleRecSub_implies_SimpleRec; assumption.
+    constructor.
+    inversion P.
+    constructor;
+    apply SimpleRecSub_implies_SimpleRec; assumption.
+
+    inversion P.
+    specialize (IHt H0).
+    apply IHt.
+
+    cbn.
+    constructor.
+    unfold comp.
+    admit.
+
+
+Admitted.
+
+    (* constructor; apply SimpleRecContr; assumption. *)
+    (* constructor. *)
+    (* constructor; apply SimpleRecContr; assumption. *)
+    (* constructor; assumption. *)
+    (* induction P. *)
+    (* cbn. *)
+    (* constructor. *)
+    (* cbn. *)
+    (* constructor. *)
+    (* apply simpl_rec_implies_rec_fu. *)
+
+    (* cbn; try constructor. *)
+    (* induction 1; cbn; constructor || intuition. *)
+
+Reserved Notation "⟪ τ ≗ τ' ⟫"
+  (at level 0, τ at level 98, τ' at level 98).
+CoInductive Tyeq : Ty → Ty → Prop :=
+| EqPrim : ⟪ tunit ≗ tunit ⟫
+| EqArr {τ τ' σ σ'} :
+    ⟪ τ ≗ σ ⟫ →
+    ⟪ τ' ≗ σ' ⟫ →
+    ⟪ tarr τ τ' ≗ tarr σ σ' ⟫
+| EqSum {τ τ' σ σ'} :
+    ⟪ τ ≗ σ ⟫ →
+    ⟪ τ' ≗ σ' ⟫ →
+    ⟪ τ ⊎ τ' ≗ σ ⊎ σ' ⟫
+| EqVar {i} :
+    ⟪ tvar i ≗ tvar i ⟫
+| EqMuL {τ σ} :
+    (* ⟪ fu' τ ≗ σ ⟫ → *)
+    ⟪ τ[beta1 (trec τ)] ≗ σ ⟫ →
+    SimpleContr τ →
+    ⟪ trec τ ≗ σ ⟫
+| EqMuR {τ σ} :
+    LMC τ = 0 →
+    SimpleContr σ →
+    ⟪ τ ≗ σ[beta1 (trec σ)] ⟫ →
+    ⟪ τ ≗ trec σ ⟫
+where "⟪ τ ≗ τ' ⟫" := (Tyeq τ τ').
+
+CoInductive Tyeq' : Ty → Ty → Prop :=
+| EqPrim' : Tyeq' tunit tunit
+| EqArr' {τ τ' σ σ'} :
+    Tyeq' τ σ →
+    Tyeq' τ' σ' →
+    Tyeq' (tarr τ τ') (tarr σ σ')
+| EqSum' {τ τ' σ σ'} :
+    Tyeq' τ σ →
+    Tyeq' τ' σ' →
+    Tyeq' (τ ⊎ τ') (σ ⊎ σ')
+| EqVar' {i} :
+    Tyeq' (tvar i) (tvar i)
+| EqMuL' {τ σ} :
+    Tyeq' (fu' (trec τ)) σ →
+    SimpleContr τ →
+    Tyeq' (trec τ) σ
+| EqMuR' {τ σ} :
+    LMC τ = 0 →
+    SimpleContr σ →
+    Tyeq' τ (fu' (trec σ)) →
+    Tyeq' τ (trec σ).
+
+
+Lemma fu_accum_subst_eq {τ ξ ζ} : SimpleContr τ → fu_accum τ (ξ >=> ζ) = fu_accum τ[ξ] ζ.
+Proof.
+  intro H.
+  revert ξ ζ.
+  induction H;
+    cbn;
+    repeat change (apTy ?ξ ?τ) with τ[ξ];
+    intros;
+    rewrite ?ap_comp;
+    try auto.
+
+  rewrite <- (IHSimpleContr ξ↑ (ζ↑ >=> beta1 (trec τ[ξ↑ >=> ζ↑]))).
+  rewrite comp_assoc.
+  rewrite comp_up.
+  reflexivity.
+Qed.
+
+Lemma fu_eq_unfold_fu {τ} : SimpleContr τ → fu' (trec τ) = fu' (τ[beta1 (trec τ)]).
+  intros.
+  unfold fu'.
+  cbn.
+  repeat change (apTy ?ξ ?τ) with τ[ξ].
+  rewrite ?ap_comp,
+  ?up_idm,
+  ?comp_id_right,
+  ?comp_id_left,
+  ?ap_id.
+
+  assert (beta1 (trec τ) = beta1 (trec τ) >=> idm Ty) by (symmetry; apply comp_id_right).
+  rewrite H0 at 1.
+  exact (@fu_accum_subst_eq τ (beta1 (trec τ)) (idm Ty) H).
+Qed.
+
+Lemma lmc_fu_zero {τ} : SimpleContr τ → LMC (fu' τ) = 0.
+Proof.
+  unfold fu'.
+  functional induction (fu_accum τ (idm Ty)) using fu_accum_ind;
+  repeat cbn; trivial.
+
+  inversion 1.
+  specialize (IHt H1).
+  assumption.
+
+  inversion 1.
+Qed.
+
+Lemma lmc_fu_zero' {τ ξ} : SimpleContr τ → LMC (fu_accum τ ξ) = 0.
+Proof.
+  revert ξ.
+  functional induction (fu_accum τ (idm Ty)) using fu_accum_ind;
+  repeat cbn; trivial.
+
+  inversion 1.
+  apply IHt.
+  assumption.
+
+  inversion 1.
+Qed.
+
+Lemma fu_id_lmc_zero {τ} : LMC τ = 0 → fu' τ = τ.
+Proof.
+  intros.
+  destruct τ; cbn; trivial; repeat change (apTy ?ξ ?τ) with τ[ξ];
+  repeat rewrite ap_id; try reflexivity.
+  enough (LMC (trec τ) <> 0) by contradiction.
+  cbn.
+  auto.
+Qed.
+
+Lemma fu_idem {τ} : SimpleContr τ → fu' (fu' (τ)) = fu' τ.
+Proof.
+  auto using fu_id_lmc_zero, lmc_fu_zero.
+Qed.
+
+Lemma fu_eq_lhs {τ} : SimpleContr τ → ⟪ fu' τ ≗ τ ⟫.
+Proof.
+  unfold fu'.
+  intro H.
+  remember (fu_accum τ (idm Ty)) as P.
+  assert (τ = τ[idm Ty]) by (symmetry; apply ap_id).
+  rewrite H0.
+  rewrite HeqP.
+  clear HeqP H0.
+  generalize (idm Ty) as ξ.
+  intro ξ.
+  functional induction (fu_accum τ ξ) using fu_accum_ind;
+    intros.
+  admit.
+  admit.
+  admit.
+  inversion H.
+  specialize (IHt H1).
+  cbn.
+  constructor.
+  apply lmc_fu_zero'.
+  assumption.
+
+
+  admit.
+Admitted.
+
+
+Lemma fu_eq_pres {τ σ} : SimpleContr τ → SimpleContr σ → ⟪ fu' τ ≗ σ ⟫ → ⟪ τ ≗ σ ⟫.
+Proof.
+  unfold fu'.
+  intros.
+  revert H1.
+
+  induction H; intros.
+  cbn in H1.
+  assumption.
+
+  cbn in H2.
+  repeat change (apTy ?ξ ?τ) with τ[ξ] in H2.
+  repeat rewrite ap_id in H2.
+  assumption.
+
+  cbn in H2.
+  repeat change (apTy ?ξ ?τ) with τ[ξ] in *.
+  repeat rewrite ap_id in H2.
+  assumption.
+
+  functional induction (fu_accum (trec τ) (idm Ty)) using fu_accum_ind.
+
+  cbn in H1.
+Admitted.
+  (* rewrite up_idm in H1. *)
+  (* rewrite comp_id_left in H1. *)
+  (* repeat change (apTy ?ξ ?τ) with τ[ξ] in *. *)
+  (* pose proof (@fu_eq_unfold_fu τ H). *)
+  (* unfold fu' in H2. *)
+  (* constructor. *)
+  (* rewrite H2 in IHSImpl *)
+  (* . *)
+
+
+
+
+
+
+  (* assert (σ = σ[idm Ty]) by (symmetry; apply ap_id). *)
+  (* rewrite H. *)
+  (* clear H. *)
+  (* generalize (idm Ty) as ξ. *)
+  (* intros. *)
+  (* functional induction (fu_accum τ ξ) using fu_accum_ind. *)
+  (* cbn in *. *)
+  (* repeat change
+ (apTy ?ξ ?τ) with τ[ξ] in *. *)
+  (* inversion H1. *)
+  (* constructor. *)
+
+Lemma fu_pres_tyeq'_lhs {τ σ} : Tyeq' τ σ → Tyeq' (fu' τ) σ.
+  intros.
+  induction τ;
+    try (
+      cbn;
+      repeat change (apTy ?ξ ?τ) with τ[ξ] in *;
+      rewrite ?ap_id;
+      assumption
+  ).
+  inversion H.
+  assumption.
+  cbn in H0.
+  lia.
+Qed.
+
+Lemma fu_pres_tyeq'_rhs {τ σ} : Tyeq' τ σ → Tyeq' τ (fu' σ).
+Proof.
+  intros.
+  induction σ;
+    try (
+      cbn;
+      repeat change (apTy ?ξ ?τ) with τ[ξ] in *;
+      rewrite ?ap_id;
+      assumption
+  ).
+  inversion H.
+  constructor.
+  inversion H0;
+    try (
+      assert (LMC (trec τ1) = LMC (fu' (trec τ0))) by (
+                                                     f_equal; assumption
+                                                   );
+      contradict H8;
+      rewrite lmc_fu_zero;
+      cbn;
+      [lia | (constructor; assumption)]
+      ).
+  all: assumption.
+Qed.
+
+Lemma fu_pres_tyeq' {τ σ} : Tyeq' τ σ → Tyeq' (fu' τ) (fu' σ).
+Proof.
+  auto using fu_pres_tyeq'_lhs, fu_pres_tyeq'_rhs.
+Qed.
+
+Lemma fuz {τ σ} : SimpleContr τ → SimpleContr σ → Tyeq' τ σ → Tyeq' (trec τ) (trec σ).
+Proof.
+  intros.
+  constructor.
+  constructor.
+  apply lmc_fu_zero.
+  constructor.
+  assumption.
+  assumption.
+  destruct τ, σ.
+  cbn.
+  repeat change (apTy ?ξ ?τ) with τ[ξ] in *.
+  rewrite ?ap_id.
+  rewrite ?
+  cbn.
+Admitted.
+
+
+
+Lemma tyeq'_refl_contr_base {τ} : SimpleContr τ → Tyeq' τ τ
+with tyeq'_refl_rec_base {τ} : SimpleRec τ → Tyeq' τ τ.
+Proof.
+  intro H.
+  induction τ;
+    try (
+      inversion H;
+      constructor;
+      auto;
+      fail
+    ).
+  constructor.
+  constructor.
+  apply lmc_fu_zero.
+  assumption.
+  inversion H.
+  assumption.
+Admitted.
+
+
+
+
+(* I have to rework this proof on paper. *)
+Lemma tyeq_refl (τ : Ty) : SimpleContr τ → ⟪ τ ≗ τ ⟫.
+Proof.
+  apply (simp_contr_mut_ind
+           (fun {τ} (_ : SimpleContr τ) => (SimpleContr τ → ⟪ τ ≗ τ ⟫))
+           (fun {τ} (_ : SimpleRec τ) => (SimpleRec τ → ⟪ τ ≗ τ ⟫)));
+    try (constructor; auto; fail).
+  intros.
+  inversion H0.
+Admitted.
+
+Lemma lhs_fu_eq (τ : Ty) (P : Contr τ) : ⟪ τ ≗ fu' τ ⟫.
+Proof.
+  unfold fu'.
+  replace τ with τ[idm Ty] at 1.
+  generalize (idm Ty).
+  induction τ;
+  cbn.
+  constructor.
+Admitted.
+
