FixIsMu/StlcIso/SpecEquivalent.v
@@ -3,16 +3,16 @@ Require Export StlcIso.SpecEvaluation.
 
 Definition PCtxEquivalent (Γ: Env) (t₁ t₂: Tm) (τ: Ty) : Prop :=
   ∀ C τ',
-    ⟪ ⊢ C : Γ , τ → empty, τ' ⟫ →
+    ⟪ i⊢ C : Γ , τ → empty, τ' ⟫ →
     (pctx_app t₁ C)⇓ ↔ (pctx_app t₂ C)⇓.
-Notation "⟪  Γ ⊢ t₁ ≃ t₂ : τ  ⟫" :=
+Notation "⟪  Γ i⊢ t₁ ≃ t₂ : τ  ⟫" :=
   (PCtxEquivalent Γ t₁ t₂ τ)
   (at level 0, Γ at level 98, t₁ at level 98, t₂ at level 98, τ at level 98).
 
 Lemma pctx_equiv_symm {Γ t₁ t₂ τ} :
-  ⟪ Γ ⊢ t₁ ≃ t₂ : τ ⟫ → ⟪ Γ ⊢ t₂ ≃ t₁ : τ ⟫.
+  ⟪ Γ i⊢ t₁ ≃ t₂ : τ ⟫ → ⟪ Γ i⊢ t₂ ≃ t₁ : τ ⟫.
 Proof.
   unfold PCtxEquivalent.
-  intros equiv C τ' ty; split;  
+  intros equiv C τ' ty; split;
   apply (equiv C τ' ty).
 Qed.
